WIP:sync

ex/exCoqRDF.v
@@ -3,15 +3,16 @@ Set Implicit Arguments.
 Unset Strict Implicit.
 Unset Printing Implicit Defensive.
 From RDF Require Export Rdf Triple Term Util.
+From Coq Require Import Strings.String.
 
 Section Sets.
 
   (* Defining some sets for IRIs, blank nodes and literals. *)
 
-  Inductive Iex :=
-  | isA
-  | Sonata
-  | Year.
+  (* Inductive Iex := *)
+  (* | isA *)
+  (* | Sonata *)
+  (* | Year. *)
 
   Inductive B1ex :=
   | A
@@ -31,16 +32,16 @@ Section Maps.
 
   (* Defining some maps resulting in the same type domain or in another one. *)
 
-  Definition mu (b: B1ex) : B1ex :=
+  Definition mu (b : nat) : nat :=
     match b with
-    | B => C
-    | _ => B
+    | 0 => 1
+    | _ => 0
     end.
 
-  Definition nu (b: B1ex) : B2ex :=
+  Definition nu (b: nat) : B1ex :=
     match b with
-    | B => F
-    | _ => E
+    | 0 => A
+    | _ => B
     end.
 
 End Maps.
@@ -50,11 +51,11 @@ Section Prelude.
 
   (* Transferring eqType infrastructure to the inductives *)
 
-  Definition eqb_i (i1 i2 : Iex) :=
-    match (i1, i2) with
-    | (isA, isA) | (Sonata,Sonata) | (Year,Year) => true
-    | (_,_) => false
-    end.
+  (* Definition eqb_i (i1 i2 : Iex) := *)
+  (*   match (i1, i2) with *)
+  (*   | (isA, isA) | (Sonata,Sonata) | (Year,Year) => true *)
+  (*   | (_,_) => false *)
+  (*   end. *)
 
   Definition eqb_b1 (b1 b2 : B1ex) :=
     match (b1, b2) with
@@ -73,7 +74,8 @@ Section Prelude.
     | ((num n), (num m)) => n == m
     end.
 
-  Lemma i_eqP : Equality.axiom eqb_i. by case; case; (try apply Bool.ReflectT=> //); apply Bool.ReflectF. Qed.
+  Lemma str_eqP : Equality.axiom String.eqb. by move=> x y; apply eqb_spec. Qed.
+  (* Lemma i_eqP : Equality.axiom eqb_i. by case; case; (try apply Bool.ReflectT=> //); apply Bool.ReflectF. Qed. *)
   Lemma b1_eqP : Equality.axiom eqb_b1. by case; case; (try apply Bool.ReflectT=> //); apply Bool.ReflectF. Qed.
   Lemma b2_eqP : Equality.axiom eqb_b2. by case; case; (try apply Bool.ReflectT=> //); apply Bool.ReflectF. Qed.
   Lemma l_eqP : Equality.axiom eqb_l.
@@ -86,10 +88,13 @@ Section Prelude.
   Qed.
 
 
-  Canonical iE := Eval hnf in EqType Iex (EqMixin i_eqP).
+  (* Canonical iE := Eval hnf in EqType Iex (EqMixin i_eqP). *)
   Canonical b1E := Eval hnf in EqType B1ex (EqMixin b1_eqP).
   Canonical b2E := Eval hnf in EqType B2ex (EqMixin b2_eqP).
   Canonical lE := Eval hnf in  EqType Lex (EqMixin l_eqP).
+  Canonical strE := Eval hnf in EqType string (EqMixin str_eqP).
+  Canonical strE := Eval hnf in EqType string (EqMixin str_eqP).
+
 
 End Prelude.
 
@@ -97,28 +102,96 @@ Section TermsEx.
 
   (* Defining some terms and testing relabeling and equality on them. *)
 
-  Definition I (i : Iex) {B : Type} := @Iri Iex B Lex i.
-  Definition L (l : Lex) {B : Type} := @Lit Iex B Lex l.
-  Definition Bn {B : Type} := @Bnode Iex B Lex.
+  (* Definition I (i : Iex) {B : Type} := @Iri Iex B Lex i. *)
+  (* Definition L (l : Lex) {B : Type} := @Lit Iex B Lex l. *)
+  (* Definition Bn {B : Type} := @Bnode Iex B Lex. *)
 
-  Definition isA1 := @I isA B1ex.
-  Definition isA2 := @I isA B2ex.
-  Definition sonata1 := @I Sonata B1ex.
-  Definition sonata2 := @I Sonata B2ex.
-  Definition year {B : Type} := @I Year B.
-  Definition b := Bn B.
-  Definition c := Bn C.
-  Definition f := Bn F.
-  Definition n1781 {B : Type} := @L (num 1781) B.
+  (* Definition isA1 := @I isA B1ex. *)
+  (* Definition isA2 := @I isA B2ex. *)
+  (* Definition sonata1 := @I Sonata B1ex. *)
+  (* Definition sonata2 := @I Sonata B2ex. *)
+  (* Definition year {B : Type} := @I Year B. *)
+  (* Definition b := Bn B. *)
+  (* Definition c := Bn C. *)
+  (* Definition f := Bn F. *)
+  (* Definition n1781 {B : Type} := @L (num 1781) B. *)
 
 
-  Example relabeling_an_iri : (relabeling_term mu isA1) == isA1. by []. Qed.
+  (* Example relabeling_an_iri : (relabeling_term mu isA1) == isA1. by []. Qed. *)
 
-  Example relabeling_a_blank_node : (relabeling_term mu b) == c. by []. Qed.
+  (* Example relabeling_a_blank_node : (relabeling_term mu b) == c. by []. Qed. *)
 
-  Example relabeling_blank_node_type : (relabeling_term nu b) == f. by []. Qed.
+  (* Example relabeling_blank_node_type : (relabeling_term nu b) == f. by []. Qed. *)
 
 End TermsEx.
+Open Scope string_scope.
+Open Scope nat_scope.
+Section TermsStr.
+
+  (* Defining some terms and testing relabeling and equality on them. *)
+  Definition iri_t := string.
+  Definition lit_t := (string * string)%type.
+  Definition I (i : iri_t) {B : Type} := @Iri iri_t B lit_t i.
+  Definition L (l : lit_t) {B : Type} := @Lit iri_t B lit_t l.
+  Definition Bn {B : Type}:= @Bnode iri_t B lit_t.
+
+  Definition isA_nat := (@I "isA" nat).
+  Definition isA_b := (@I "isA" B1ex).
+  Definition sonata := (@I "sonata" nat).
+  Definition sonata_b := (@I "sonata" B1ex).
+  Definition year {B : Type} := @I "year" B.
+  (* Definition year {B : Type} := @I Year B. *)
+  Definition a := Bn A.
+  Definition z := Bn 0.
+  Definition f := Bn 5.
+  Definition n1781 {B : Type} := @L ("number","1781") B.
+
+
+  Example relabeling_an_iri : (relabeling_term mu (@I "isA" nat)) == (@I "isA" nat). by []. Qed.
+
+  Example relabeling_a_blank_node : (relabeling_term mu (Bn 0)) == (Bn 1). by []. Qed.
+
+  Example relabeling_blank_node_type : (relabeling_term nu (Bn 0)) == (Bn A). by []. Qed.
+
+End TermsStr.
+Section TripleStr.
+
+  (* Defining some triples and testing relabeling and equality on them. *)
+
+  Definition mkTriple {B : Type} := @mkTriple iri_t B lit_t.
+
+  (* type aliases *)
+  Definition tr_b1 := triple strE nat lit_t.
+  Definition tr_b2 := triple strE b1E lit_t.
+
+  Definition z_isA_sonata : tr_b1. by refine (@mkTriple _ z isA_nat sonata _ _). Defined.
+  Definition a_isA_sonata : tr_b2. by refine (@mkTriple _ (Bn A) isA_b sonata_b _ _). Defined.
+  Definition o_isA_sonata : tr_b1. by refine (@mkTriple _ (Bn 1) isA_nat sonata _ _). Defined.
+  Definition a_year_1781 : tr_b2. by refine (@mkTriple _ a year n1781 _ _). Defined.
+  Definition o_year_1781 : tr_b1. by refine (@mkTriple _ (Bn 1) year n1781 _ _). Defined.
+
+  Example relabeling_a_triple_eq : relabeling_triple mu z_isA_sonata == o_isA_sonata. by []. Qed.
+
+  Example relabeling_a_triple_neq : relabeling_triple nu z_isA_sonata == a_year_1781 = false. by []. Qed.
+
+End TripleStr.
+Section GraphStr.
+  (* Defining some graphs and testing relabeling and equality on them. *)
+
+  (* type aliases *)
+  Definition RDF_b1 := rdf_graph strE nat_eqType lit_t.
+  Definition RDF_b2 := rdf_graph strE b1E lit_t.
+
+  Definition BSonataG : RDF_b1. by refine (@mkRdfGraph _ _ _ [:: b_isA_sonata; b_year_1781] _). Defined.
+  Definition relabeled_G : RDF_b2. by refine (@relabeling _ _ _ _ nu BSonataG _). Defined.
+  Definition BSonataG_perm : RDF_b1. by refine (@mkRdfGraph _ _ _ [:: b_year_1781 ; b_isA_sonata ] _). Defined.
+  Definition FSonataG : RDF_b2. by refine (@mkRdfGraph _ _ _ [:: f_isA_sonata; f_year_1781] _). Defined.
+
+  Example graphs_eq : eqb_rdf BSonataG BSonataG_perm. by []. Qed.
+  Example graphs_relabel_eq : eqb_rdf relabeled_G FSonataG. by []. Qed.
+  Example graphs_prop_neq : BSonataG == empty_rdf_graph = false. by []. Qed.
+
+End GraphEx.
 
 Section TripleEx.
 
